%\chapter{Infinite sequences and series}
\graphicspath{{./chap1/images/}}   

%\section{Introduction}
The identity we need to prove is
\begin{align}
    \zeta(2) = \sum_{n=0}^\infty \frac{1}{n^2} = \frac{\pi^2}{6} \tag{1}\label{eq:1}
\end{align}
Since it is clear that
\[
    \frac{3}{4}\zeta(2) = \sum_{n=0}^\infty \frac{1}{n^2} -  \sum_{m=0}^\infty \frac{1}{(2m)^2}= \sum_{r=0}^\infty \frac{1}{(2r+1)^2} 
\]
\eqref{eq:1} is equivalent with
\begin{align}
    \sum_{r=0}^\infty \frac{1}{(2r+1)^2} = \frac{\pi^2}{8} \tag{2}\label{eq:2}
\end{align}
\section{Series}
\section{Geometric series}
\section{The nth term test}
\section{Combining series}
\section{Adding or deleting terms}
\section{Re-indexing terms}